template-coq/theories/kernel/uGraph.v
@@ -1,170 +1,365 @@
-Require Import BinInt List. Import ListNotations.
-From Template Require Import config Universes.
-
-
-
-(* Prop < Set <= other levels *)
-(* Each time a level l is inserted in the graph, the constraint *)
-(* Set <= l is added. *)
-
-(* For the moment we recompute the graph each time *)
-(* TODO the first component is useless *)
-Definition t : Type := LevelSet.t * ConstraintSet.t.
-
-(* TODO use nat where Z is not useful or BinNat *)
+Require Import Bool String BinInt List Relations. Import ListNotations.
+Require MSets.MSetWeakList.
+From Template Require Import utils config Universes.
+Import ConstraintType.
 Local Open Scope Z.
 
-Definition edge : Set := Level.t * Z * Level.t.
+(* vertices of the graph are levels which are not Prop *)
+Inductive vertice := lSet | Level (_ : string) | Var (_ : nat).
 
-Definition edges_of_constraint (uc : univ_constraint) : list edge
-  := let '((l, ct),l') := uc in
-     match ct with
-     | ConstraintType.Lt => [(l,-1,l')]
-     | ConstraintType.Le => [(l,0,l')]
-     | ConstraintType.Eq => [(l,0,l'); (l',0,l)]
-     end.
-
-Definition init_graph : t :=
-  let levels := LevelSet.add Level.prop (LevelSet.add Level.set LevelSet.empty) in
-  let constraints := ConstraintSet.add (Level.prop, ConstraintType.Lt, Level.set) ConstraintSet.empty in
-  (levels, constraints).
-
-(* The monomorphic levels are > Set while polymorphic ones are >= Set. *)
-Definition add_node (l : Level.t) (G : t) : t
-  := let levels := LevelSet.add l (fst G) in
-     let constraints :=
-         match l with
-         | Level.lProp | Level.lSet => snd G (* supposed to be yet here *)
-         | Level.Var _ => ConstraintSet.add (Level.set, ConstraintType.Le, l) (snd G)
-         | Level.Level _ => ConstraintSet.add (Level.set, ConstraintType.Lt, l) (snd G)
-         end in
-     (levels, constraints).
-
-Definition add_constraint (uc : univ_constraint) (G : t) : t
-  := let '((l, ct),l') := uc in
-     (* maybe useless if we always add constraints
-        in which the universes are declared *)
-     let G := add_node l (add_node l' G) in
-     let constraints := ConstraintSet.add uc (snd G) in
-     (fst G, constraints).
-
-Definition repr (uctx : universe_context) : UContext.t :=
-  match uctx with
-  | Monomorphic_ctx c => c
-  | Polymorphic_ctx c => c
-  | Cumulative_ctx c => CumulativityInfo.univ_context c
+(* vertive to level *)
+Definition vtl (v : vertice) : Level.t :=
+  match v with
+  | lSet => Level.lSet
+  | Level x => Level.Level x
+  | Var x => Level.Var x
   end.
 
-Definition add_global_constraints (uctx : universe_context) (G : t) : t
-  := match uctx with
-     | Monomorphic_ctx (inst, cstrs) =>
-       let G := List.fold_left (fun s l => add_node l s) inst G in
-       ConstraintSet.fold add_constraint cstrs G
-     | Polymorphic_ctx _ => G
-     | Cumulative_ctx _ => G
+(* level to vertice *)
+Definition ltv (l : universe_level) : option vertice :=
+  match l with
+  | Level.lProp => None
+  | Level.lSet => Some lSet
+  | Level.Level x => Some (Level x)
+  | Level.Var x => Some (Var x)
+  end.
+
+(* true is for 0, false for -1 *)
+Definition edge : Set := vertice * bool * vertice.
+
+(* bool to Z *)
+Definition btz (b : bool) : Z := if b then 0 else -1.
+
+Module VerticeDec.
+  Definition t : Set := vertice.
+  Definition eq : t -> t -> Prop := eq.
+  Definition eq_equiv : RelationClasses.Equivalence eq := _.
+  Definition eq_refl : forall x : t, eq x x := @eq_refl _.
+  Definition eq_sym : forall x y : t, eq x y -> eq y x := @eq_sym _.
+  Definition eq_trans : forall x y z : t, eq x y -> eq y z -> eq x z := @eq_trans _.
+  Definition eq_dec : forall x y : t, {eq x y} + {~ eq x y}.
+    unfold eq.
+    decide equality. apply string_dec. apply Peano_dec.eq_nat_dec.
+  Defined.
+End VerticeDec.
+Module VerticeSet <: MSetInterface.WSetsOn VerticeDec := MSets.MSetWeakList.Make VerticeDec.
+Module VerticeMap := FSets.FMapWeakList.Make VerticeDec.
+
+Module EdgeDec.
+  Definition t : Set := edge.
+  Definition eq : t -> t -> Prop := eq.
+  Definition eq_equiv : RelationClasses.Equivalence eq := _.
+  Definition eq_dec : forall x y : t, {eq x y} + {~ eq x y}.
+    unfold eq.
+    decide equality. apply VerticeDec.eq_dec.
+    decide equality. apply Bool.bool_dec.
+    (* apply ZArith_dec.Z_eq_dec. *)
+    apply VerticeDec.eq_dec.
+  Defined.
+End EdgeDec.
+Module EdgeSet <: MSetInterface.WSetsOn EdgeDec := MSets.MSetWeakList.Make EdgeDec.
+
+(* If [None] the constraint is inconsistent *)
+(* If [Some empty] the constraint is useless *)
+(* Set < l or Set <= l are supposed to be yet present in the graph *)
+Definition edges_of_constraint (uc : univ_constraint) : option EdgeSet.t
+  := let '(l1, t, l2) := uc in
+     match ltv l1, t, ltv l2 with
+     (* l <= Prop or l < Prop or l = Prop *)
+     | _, _, None => None
+     (* Prop <= l *)
+     | None, Le, _ => Some EdgeSet.empty
+     (* Prop = l *)
+     | None, Eq, _ => None
+     (* Prop < l  ->  idem as Set <= l *)
+     | None, Lt, _ => Some EdgeSet.empty
+
+     | Some lSet, Eq, Some (Level _) => None
+     | Some (Level _), Eq, Some lSet => None
+     | _, Lt, Some lSet => None
+     | Some lSet, Le, Some _ => Some EdgeSet.empty
+
+     | Some l, Le, Some l' => Some (EdgeSet.singleton (l, true, l'))
+     | Some l, Lt, Some l' => Some (EdgeSet.singleton (l, false, l'))
+     | Some l, Eq, Some l' => Some (EdgeSet.add (l', true, l) (EdgeSet.singleton (l, true, l')))
      end.
 
-Section UGraph.
-  Variable (φ : t).
+     (* (* l <= Prop or l < Prop or l = Prop *) *)
+     (* | _, _, Level.lProp => None *)
+     (* (* Prop <= l *) *)
+     (* | (Level.lProp, Le, _) => Some EdgeSet.empty *)
+     (* (* Prop = l *) *)
+     (* | (Level.lProp, Eq, _) => None *)
+     (* (* Prop < l  ->  idem as Set <= l *) *)
+     (* | (Level.lProp, Lt, _) => Some EdgeSet.empty *)
 
-  (* FIXME duplicates *)
-  Definition edges : list edge
-    := ConstraintSet.fold (fun uc E => edges_of_constraint uc ++ E) (snd φ) [].
+     (* (* Set <= l *) *)
+     (* | (Level.lSet, Le, _) => Some EdgeSet.empty *)
+     (* (* Set < l *) *)
+     (* | (Level.lSet, Lt, Level.lSet) => None *)
+     (* | (Level.lSet, Lt, Level.Level _) => Some EdgeSet.empty *)
+     (* | (Level.lSet, Lt, Level.Var x) => Some (EdgeSet.singleton (lSet, true, Var x)) *)
+     (* (* Set = l *) *)
+     (* | (Level.lSet, Eq, Level.lSet) => Some EdgeSet.empty *)
+     (* | (Level.lSet, Eq, Level.Level _) => None *)
+     (* | (Level.lSet, Eq, Level.Var x) => Some (EdgeSet.singleton (Var x, true, lSet)) *)
+     (* (* l <= Set *) *)
+     (* | (Level.Level l, Le, Level.lSet) =>  Some (EdgeSet.singleton (Level l, true, lSet)) *)
+     (* | (Level.Var l, Le, Level.lSet) =>  Some (EdgeSet.singleton (Var l, true, lSet)) *)
+     (* (* l < Set *) *)
+     (* | (_, Lt, Level.lSet) => None *)
+     (* (* l = Set *) *)
+     (* | (Level.Level _, Eq, Level.lSet) =>  None *)
+     (* | (Level.Var l, Eq, Level.lSet) =>  Some (EdgeSet.singleton (Var l, true, lSet)) *)
+                                            
+     (* (* l <= l' *) *)
+     (* | (Level.Level l, Le, Level.Level l') =>  Some (EdgeSet.singleton (Level l, true, Level l')) *)
+     (* | (Level.Var l, Le, Level.Level l') =>  Some (EdgeSet.singleton (Var l, true, Level l')) *)
+     (* | (Level.Level l, Le, Level.Var l') =>  Some (EdgeSet.singleton (Level l, true, Var l')) *)
+     (* | (Level.Var l, Le, Level.Var l') =>  Some (EdgeSet.singleton (Var l, true, Var l')) *)
+     (* (* l < l' *) *)
+     (* | (Level.Level l, Lt, Level.Level l') =>  Some (EdgeSet.singleton (Level l, false, Level l')) *)
+     (* | (Level.Var l, Lt, Level.Level l') =>  Some (EdgeSet.singleton (Var l, false, Level l')) *)
+     (* | (Level.Level l, Lt, Level.Var l') =>  Some (EdgeSet.singleton (Level l, false, Var l')) *)
+     (* | (Level.Var l, Lt, Level.Var l') =>  Some (EdgeSet.singleton (Var l, false, Var l')) *)
 
-  (* The graph *)
-  (* For each node we record its predecessos  *)
-  Definition pred_graph := LevelMap.t (Level.t * Z).
+     (* (* l = l' *) *)
+     (* | (Level.Level l, Eq, Level.Level l') =>  Some (EdgeSet.add (Level l', true, Level l) (EdgeSet.singleton (Level l, true, Level l'))) *)
+     (* | (Level.Var l, Eq, Level.Level l') =>  Some (EdgeSet.add (Level l', true, Var l) (EdgeSet.singleton (Var l, true, Level l'))) *)
+     (* | (Level.Level l, Eq, Level.Var l') =>  Some (EdgeSet.add (Var l', true, Level l) (EdgeSet.singleton (Level l, true, Var l'))) *)
+     (* | (Level.Var l, Eq, Level.Var l') =>  Some (EdgeSet.add (Var l', true, Var l) (EdgeSet.singleton (Var l, true, Var l'))) *)
+     (* end. *)
 
-  Definition Zinfty := (Z.pow 2 6)%Z.  (* FIXME bigger at least *)
+(* If [None] the set of constraints is naively inconsistent *)
+Definition edges_of_constraints (ctrs : constraints) : option EdgeSet.t :=
+  ConstraintSet.fold (fun uc S => match edges_of_constraint uc, S with
+                               | Some S1, Some S2 => Some (EdgeSet.union S1 S2)
+                               | _, _ => None end) ctrs (Some EdgeSet.empty).
 
-  Definition add_node_pred_graph l := LevelMap.add l (Level.Level "nil", Zinfty).
 
-  Definition init_pred_graph : pred_graph :=
-    LevelSet.fold add_node_pred_graph (fst φ) (LevelMap.empty _).
+(* Prop is never in the graph *)
+(* Nodes of the graph are nodes of the constraints + Set *)
+(* For each universe, at least the constraint l > Set or l >= Set is here *)
+Definition t  := VerticeSet.t × EdgeSet.t.
 
-  Definition relax (G : pred_graph) (e : edge) : pred_graph :=
+Definition init_graph : t :=
+  (VerticeSet.singleton lSet, EdgeSet.empty).
+
+(* without Prop nor Set *)
+Definition nodes_of_level (l : universe_level) : VerticeSet.t :=
+  match ltv l with
+  | None => VerticeSet.empty
+  | Some l=> VerticeSet.singleton l
+  end.
+
+Definition nodes_of_constraint (ctr : univ_constraint) : VerticeSet.t :=
+  let '(l1, _, l2) := ctr in
+  VerticeSet.union (nodes_of_level l1) (nodes_of_level l2).
+
+Definition add_nodes_of_constraints (ctrs : constraints) :=
+  ConstraintSet.fold (fun ctr => VerticeSet.union (nodes_of_constraint ctr)) ctrs.
+
+(* If [None] the set of constraints is naively inconsistent *)
+Definition make_graph (ctrs : constraints) : option t
+  := let V := add_nodes_of_constraints ctrs (VerticeSet.singleton lSet) in
+     let E0 := VerticeSet.fold (fun v S => match v with
+                                 | Level l => EdgeSet.add (lSet, false, Level l) S
+                                 | Var l => EdgeSet.add (lSet, true, Var l) S
+                                 | _ => S end) V EdgeSet.empty in
+     match edges_of_constraints ctrs with
+     | Some E1 => Some (V, EdgeSet.union E0 E1)
+     | None => None
+     end.
+
+Section Graph.
+  Context (φ : t).
+
+  Inductive R0s : vertice -> vertice -> Prop :=
+  | R00 l : R0s l l
+  | R01 l1 l2 l3 : R0s l1 l2 -> EdgeSet.In (l2,true,l3) (snd φ) -> R0s l1 l3.
+
+  Inductive R : vertice -> vertice -> Prop :=
+  | Rintro l1 l2 l3 l4 : R0s l1 l2 -> EdgeSet.In (l2,false,l3) (snd φ)
+                         -> R0s l3 l4 -> R l1 l4.
+
+  Definition acyclic := forall l, Acc R l.
+
+  Definition Rs : relation vertice :=
+    clos_trans _ (fun l l' => EdgeSet.In (l, true, l') (snd φ)
+                           \/ EdgeSet.In (l, false, l') (snd φ)).
+  
+  Conjecture R_dec : forall x y, {R x y} + {~ R x y}.
+  Conjecture Rs_dec : forall x y, {Rs x y} + {~ Rs x y}.
+
+  Fixpoint preds l (L : list vertice) : list {l' & R l' l} :=
+    match L with
+    | [] => []
+    | l' :: L => match R_dec l' l with
+                | left p => (existT _ _ p) :: (preds l L)
+                | right _ => preds l L
+                end
+    end.
+
+  Definition d (s l : vertice) (H : Acc R l) : option Z.
+    destruct (Rs_dec s l) as [_|_]; [apply Some|apply None].
+    induction H as [l H d].
+    simple refine (let preds := preds l (VerticeSet.elements (fst φ)) in _).
+    exact (List.fold_left (fun n X => Z.min n (d X.1 X.2)) preds 0).
+  Defined.
+
+End Graph.  
+
+Definition is_Some {A} (x : option A) := exists a, x = Some a.
+
+Conjecture Acc_ok : forall ctrs, consistent ctrs <-> exists φ, make_graph ctrs = Some φ /\ well_founded (R φ).
+Conjecture d_ok   : forall ctrs φ (e : make_graph ctrs = Some φ) (H : well_founded (R φ)) l l',
+    (exists k, forall v, satisfies v ctrs -> (val0 v (vtl l) <= (val0 v (vtl l')) + k)%Z)
+    <-> is_Some (d φ l l' (H _)).
+Conjecture d_ok2  : forall ctrs φ (e : make_graph ctrs = Some φ) (H : well_founded (R φ)) l l' k,
+    (forall v, satisfies v ctrs -> (val0 v (vtl l) <= (val0 v (vtl l')) + k)%Z)
+    <-> (forall k', d φ l l' (H _) = Some k' -> k >= k').
+
+
+
+
+Section BellmanFord.
+
+  Context (φ : t).
+
+  (* Z ∪ +∞ *)
+  (* None is for +∞ *)
+  Definition Zbar := Z.
+
+  (* For each node: predecessor and distance from the source *)
+  Definition pred_graph := VerticeMap.t (vertice * Zbar).
+
+  (* Definition add_node_pred_graph n : pred_graph -> pred_graph *)
+  (* := VerticeMap.add n None. *)
+
+  Definition init_pred_graph s : pred_graph :=
+    (* let G := EdgeSet.fold *)
+    (* (fun '(l1,_,l2) G => add_node_pred_graph l2 (add_node_pred_graph l1 G)) *)
+    (* φ (VerticeMap.empty _) in *)
+    VerticeMap.add s (s, 0) (VerticeMap.empty _).
+
+  Definition relax (e : edge) (G : pred_graph) : pred_graph :=
     let '((u, w), v) := e in
-    match LevelMap.find u G, LevelMap.find v G with
-    | Some (_, ud), Some (_, vd)
-      => if vd >=? (ud + w) then
-          LevelMap.add v (u, ud + w) G
-        else G
+    match VerticeMap.find u G, VerticeMap.find v G with
+    | Some (_, ud), Some (_, vd) => if vd >? (ud + btz w) then
+                                     VerticeMap.add v (u, ud + btz w) G
+                                   else G
+    | Some (_, ud), None => VerticeMap.add v (u, ud + btz w) G
     | _, _ => G
     end.
 
-  Definition BellmanFord (G : pred_graph) (s : Level.t) : pred_graph :=
-    let G' := LevelMap.add s (Level.Level "nil", Z0) G in
-    let G' := LevelMap.fold (fun _ _ => fold_left relax edges) G G' in
+  Definition BellmanFord s : pred_graph :=
+    let G := init_pred_graph s in
+    let G' := VerticeSet.fold (fun _ => EdgeSet.fold relax (snd φ)) (fst φ) G in
     G'.
 
-  (* true if there is a negative cycle *)
-  Definition detect_negative_cycle (G : pred_graph) : bool
-    := existsb (fun '((u,w),v) =>
-                  match LevelMap.find u G, LevelMap.find v G with
-                  | Some (_, ud), Some (_, vd)
-                    => Z.gtb vd (ud + w)
-                  | _, _ => false
-                  end) edges.
+  (* true if all is ok *)
+  Definition no_universe_inconsistency : bool :=
+    let G := BellmanFord lSet in
+    let negative_cycle := EdgeSet.exists_ (fun '((u,w),v) =>
+                          match VerticeMap.find u G, VerticeMap.find v G with
+                          | Some (_, ud), Some (_, vd) => Z.gtb vd (ud + btz w)
+                          | _, _ => false
+                          end) (snd φ) in
+    negb negative_cycle.
+
+  (** *** Universe comparisons *)
 
   (* If enforce l1 l2 = Some n, the graph enforces that l2 is at least l1 + n *)
   (* i.e. l1 + n <= l2 *)
   (* If None nothing is enforced by the graph between those two levels *)
-  Definition enforce (u v : Level.t) : option Z :=
-    let G := BellmanFord init_pred_graph u in
-    match LevelMap.find v G with
+  Definition enforce (u v : vertice) : option Z :=
+    let G := BellmanFord u in
+    match VerticeMap.find v G with
     | Some (_, vd) => Some (Z.opp vd)
     | None => None
     end.
-  Definition check_le_level (l1 l2 : Level.t) : bool :=
+
+  Definition check_le_vertice (l1 l2 : vertice) : bool :=
     match enforce l1 l2 with
     | Some k => Z.geb k 0
     | None => false
     end.
 
-  Definition check_lt_level (l1 l2 : Level.t) : bool :=
+  Definition check_lt_vertice (l1 l2 : vertice) : bool :=
     match enforce l1 l2 with
     | Some k => Z.geb k 1
     | None => false
     end.
 
-  Definition check_eq_level (l1 l2 : Level.t) : bool :=
+  Definition check_eq_vertice (l1 l2 : vertice) : bool :=
+    check_le_vertice l1 l2 && check_le_vertice l2 l1.
+
+
+  Definition check_le_level (l1 l2 : universe_level) : bool :=
+    match ltv l1, ltv l2 with
+    | None, _ => true
+    | _, None => false
+    | Some l1, Some l2 => match enforce l1 l2 with
+                         | Some k => Z.geb k 0
+                         | None => false
+                         end
+    end.
+
+  Definition check_lt_level (l1 l2 : universe_level) : bool :=
+    match ltv l1, ltv l2 with
+    | _, None => false
+    | None, _ => true
+    | Some l1, Some l2 => match enforce l1 l2 with
+                         | Some k => Z.geb k 1
+                         | None => false
+                         end
+    end.
+
+  Definition check_eq_level (l1 l2 : universe_level) : bool :=
     check_le_level l1 l2 && check_le_level l2 l1.
 
 
-  Definition check_constraint (cstr : univ_constraint) :=
+  Definition check_constraint (cstr : univ_constraint) : bool :=
     let '(l, d, r) := cstr in
     match d with
-    | ConstraintType.Eq => check_eq_level l r
-    | ConstraintType.Lt => check_lt_level l r
-    | ConstraintType.Le => check_le_level l r
+    | Eq => check_eq_level l r
+    | Lt => check_lt_level l r
+    | Le => check_le_level l r
     end.
 
-  Definition check_constraints (cstrs : ConstraintSet.t) :=
+  Definition check_constraints (cstrs : ConstraintSet.t) : bool :=
     ConstraintSet.for_all check_constraint cstrs.
 
   Definition check_le_level_expr (e1 e2 : Universe.Expr.t) : bool :=
-    match e1, e2 with
-    | (l1, false), (l2, false)
-    | (l1, true), (l2, true) => check_le_level l1 l2
-    | (l1, true), (l2, false) => check_lt_level l1 l2
-    | (l1, false), (l2, true) => match enforce l1 l2 with
-                               | Some k => Z.geb k (-1)
-                               | _ => false
-                               end
+    match ltv (fst e1), ltv (fst e2) with
+    | None, _ => true
+    | _, None => false
+    | Some l1, Some l2 =>
+      match enforce l1 l2 with
+      | None => false
+      | Some k => match snd e1, snd e2 with
+                 | false, false
+                 | true, true => k >=? 0
+                 | true, false => k >=? 1
+                 | false, true => k >=? -1
+                 end
+      end
     end.
 
   Definition check_lt_level_expr (e1 e2 : Universe.Expr.t) : bool :=
-    match e1, e2 with
-    | (l1, false), (l2, false)
-    | (l1, true), (l2, true) => check_lt_level l1 l2
-    | (l1, true), (l2, false) => match enforce l1 l2 with
-                               | Some k => Z.geb k 1 (* Approximation? *)
-                               | _ => false
-                               end
-    | (l1, false), (l2, true) => match enforce l1 l2 with
-                               | Some k => Z.geb k 0 (* Approximation ? *)
-                               | _ => false
-                               end
+    match ltv (fst e1), ltv (fst e2) with
+    | _, None => false
+    | None, _ => true
+    | Some l1, Some l2 =>
+      match enforce l1 l2 with
+      | None => false
+      | Some k => match snd e1, snd e2 with
+                 | false, false
+                 | true, true => k >=? 1
+                 | true, false => k >=? 2
+                 | false, true => k >=? 0
+                 end
+      end
     end.
 
   Definition check_eq_level_expr (e1 e2 : Universe.Expr.t) : bool :=
@@ -176,86 +371,184 @@ Section UGraph.
   Definition exists_strictly_bigger (e1 : Universe.Expr.t) (u2 : Universe.t) : bool :=
     Universe.existsb (check_lt_level_expr e1) u2.
 
-  Definition check_leq `{cf : checker_flags} (u1 u2 : Universe.t) : bool :=
-    (negb check_univs) || Universe.for_all (fun e => exists_bigger_or_eq e u2) u1.
-
   Definition check_lt (u1 u2 : Universe.t) : bool :=
     Universe.for_all (fun e => exists_strictly_bigger e u2) u1.
 
-  (* true if all is ok *)
-  Definition no_universe_inconsistency : bool :=
-    let G := BellmanFord init_pred_graph Level.prop in
-    negb (detect_negative_cycle G).
+  Definition check_leq0 (u1 u2 : Universe.t) : bool :=
+    Universe.for_all (fun e => exists_bigger_or_eq e u2) u1.
 
-End UGraph.
+  (** We try syntactic equality before checking the graph. *)
+  Definition check_leq `{checker_flags} s s' :=
+    negb check_univs || Universe.equal s s' || check_leq0 s s'.
 
+  Definition check_eq `{checker_flags} s s' :=
+    negb check_univs || Universe.equal s s' || (check_leq0 s s' && check_leq0 s' s).
 
-(* Section Test. *)
+  Definition check_eq_instance `{checker_flags} u v :=
+    Instance.equal_upto check_eq_level u v.
 
-(*   Compute init_graph. *)
-
-(*   Definition G := init_graph. *)
-
-(*   Compute (check_leq G Universe.type0m Universe.type0). *)
-(*   Compute (check_lt G Universe.type0m Universe.type0). *)
-(*   Compute (check_lt G Universe.type0m Universe.type0m). *)
-(*   Compute (check_lt G Universe.type0 Universe.type0m). *)
-(*   Compute (check_lt G Universe.type0 Universe.type0). *)
-(*   Compute (no_universe_inconsistency G). *)
-
-(*   Definition G' := add_constraint (Level.Level "Top.0", Lt, Level.Level "Top.1") *)
-(*                        (add_constraint (Level.Var 0, Lt, Level.Var 1) G). *)
-
-(*   Compute (check_lt G' (Universe.make (Level.Level "Top.0")) (Universe.make (Level.Var 0))). *)
-(*   Compute (check_leq G' (Universe.make (Level.Level "Top.1")) (Universe.make (Level.lProp))). *)
-(*   Compute (check_leq G' (Universe.super (Level.Level "Top.1")) (Universe.make (Level.Level "Top.1"))). *)
-(*   Compute (check_lt G' (Universe.make (Level.Level "Top.1")) (Universe.super (Level.Level "Top.1"))). *)
-(*   Compute (check_lt G' (Universe.make (Level.Level "Top.1")) (Universe.make (Level.Level "Top.1"))). *)
+End BellmanFord.
 
 
-(*   Compute G'. *)
-(*   Compute (no_universe_inconsistency G'). *)
-(*   Compute (check_lt G' (Universe.make (Level.Var 1)) (Universe.make (Level.Var 0))). *)
-(*   Compute (check_leq G' (Universe.make (Level.Var 0)) (Universe.make (Level.Var 1))). *)
-(*   Compute (check_lt G' (Universe.make (Level.Var 0)) (Universe.make (Level.Var 1))). *)
+Section Specif.
+  Conjecture no_universe_inconsistency_ok : forall φ, reflect (well_founded (R φ)) (no_universe_inconsistency φ).
 
-(*   Compute (check_leq G' Universe.type1 Universe.type0). *)
-(*   Compute (check_lt G' Universe.type1 Universe.type1). *)
+  Local Existing Instance default_checker_flags.
 
+  (* TODO: lower level conjecture *)
+  Conjecture check_leq_specif
+    : forall ctrs φ (e : make_graph ctrs = Some φ) u1 u2, reflect (leq_universe ctrs u1 u2) (check_leq φ u1 u2).
 
-(*   Definition G'' := add_constraint (Level.Var 1, Lt, Level.Var 2) *)
-(*                                   (add_constraint (Level.Var 2, Lt, Level.lSet) G'). *)
+  Conjecture check_eq_specif
+    : forall ctrs φ (e : make_graph ctrs = Some φ) u1 u2, reflect (eq_universe ctrs u1 u2) (check_eq φ u1 u2).
+End Specif.
 
-(*   Compute (no_universe_inconsistency G''). *)
+  (* Definition check_eq_refl `{checker_flags} u : check_eq φ u u = true. *)
+  (*   unfold check_eq; destruct check_univs; cbn; [|reflexivity]. *)
 
-(* End Test. *)
-
-(** *** Universe comparisons *)
-
-(** We try syntactic equality before checking the graph. *)
-
-Require Import Bool.
-
-Definition eq_universe `{checker_flags} φ s s' :=
-  if Universe.equal s s' then true
-  else check_leq φ s s' && check_leq φ s' s.
-
-Definition leq_universe `{checker_flags} φ s s' :=
-  if Universe.equal s s' then true
-  else check_leq φ s s'.
-
-Definition eq_universe_instance `{checker_flags} φ u v :=
-  Instance.equal_upto (check_eq_level φ) u v.
-
-Conjecture eq_universe_refl : forall `{checker_flags} φ u, eq_universe φ u u = true.
-Conjecture eq_universe_instance_refl : forall `{checker_flags} φ u, eq_universe_instance φ u u = true.
-Conjecture eq_universe_leq_universe : forall `{checker_flags} φ x y,
-    eq_universe φ x y = true -> leq_universe φ x y = true.
-Conjecture leq_universe_product_l : forall `{checker_flags} φ s1 s2,
-    leq_universe φ s1 (Universe.sort_of_product s1 s2) = true.
-Conjecture leq_universe_product_r : forall `{checker_flags} φ s1 s2,
-    leq_universe φ s2 (Universe.sort_of_product s1 s2) = true.
+  (* Conjecture eq_universe_instance_refl : forall `{checker_flags} u, eq_universe_instance u u = true. *)
+  (* Conjecture eq_universe_leq_universe : forall `{checker_flags} x y, *)
+  (*     eq_universe x y = true -> leq_universe x y = true. *)
+  (* Conjecture leq_universe_product_l : forall `{checker_flags} s1 s2, *)
+  (*     leq_universe s1 (Universe.sort_of_product s1 s2) = true. *)
+  (* Conjecture leq_universe_product_r : forall `{checker_flags} s1 s2, *)
+  (*     leq_universe s2 (Universe.sort_of_product s1 s2) = true. *)
 
 
-Definition graph_of_constraints (φ : constraints) : t
-  := ConstraintSet.fold add_constraint φ init_graph.
+
+
+    (* Inductive super_result := *)
+    (* | SuperSame (_ : bool) *)
+    (* (* The level expressions are in cumulativity relation. boolean *)
+    (*        indicates if left is smaller than right?  *) *)
+    (* | SuperDiff (_ : comparison). *)
+    (* (* The level expressions are unrelated, the comparison result *)
+    (*        is canonical *) *)
+
+    (* (** [super u v] compares two level expressions, *)
+    (*    returning [SuperSame] if they refer to the same level at potentially different *)
+    (*    increments or [SuperDiff] if they are different. The booleans indicate if the *)
+    (*    left expression is "smaller" than the right one in both cases. *) *)
+    (* Definition super (x y : t) : super_result := *)
+    (*   match Level.compare (fst x) (fst y) with *)
+    (*   | Eq => SuperSame (bool_lt' (snd x) (snd y)) *)
+    (*   | cmp => *)
+    (*       match x, y with *)
+    (*       | (l, false), (l', false) => *)
+    (*         match l, l' with *)
+    (*         | Level.lProp, Level.lProp => SuperSame false *)
+    (*         | Level.lProp, _ => SuperSame true *)
+    (*         | _, Level.lProp => SuperSame false *)
+    (*         | _, _ => SuperDiff cmp *)
+    (*         end *)
+    (*       | _, _ => SuperDiff cmp *)
+    (*       end *)
+    (*   end. *)
+
+
+  (* Fixpoint merge_univs (fuel : nat) (l1 l2 : list Expr.t) : list Expr.t := *)
+  (*   match fuel with *)
+  (*   | O => l1 *)
+  (*   | S fuel => match l1, l2 with *)
+  (*              | [], _ => l2 *)
+  (*              | _, [] => l1 *)
+  (*              | h1 :: t1, h2 :: t2 => *)
+  (*                match Expr.super h1 h2 with *)
+  (*                | Expr.SuperSame true (* h1 < h2 *) => merge_univs fuel t1 l2 *)
+  (*                | Expr.SuperSame false => merge_univs fuel l1 t2 *)
+  (*                | Expr.SuperDiff Lt (* h1 < h2 is name order *) *)
+  (*                  => h1 :: (merge_univs fuel t1 l2) *)
+  (*                | _ => h2 :: (merge_univs fuel l1 t2) *)
+  (*                end *)
+  (*              end *)
+  (*   end. *)
+
+
+
+(* (* The monomorphic levels are > Set while polymorphic ones are >= Set. *) *)
+(* Definition add_node (l : Level.t) (G : t) : t *)
+(*   := let levels := LevelSet.add l (fst G) in *)
+(*      let constraints := *)
+(*          match l with *)
+(*          | Level.lProp | Level.lSet => snd G (* supposed to be yet here *) *)
+(*          | Level.Var _ => ConstraintSet.add (Level.set, ConstraintType.Le, l) (snd G) *)
+(*          | Level.Level _ => ConstraintSet.add (Level.set, ConstraintType.Lt, l) (snd G) *)
+(*          end in *)
+(*      (levels, constraints). *)
+
+(* Definition add_constraint (uc : univ_constraint) (G : t) : t *)
+(*   := let '((l, ct),l') := uc in *)
+(*      (* maybe useless if we always add constraints *)
+(*         in which the universes are declared *) *)
+(*      let G := add_node l (add_node l' G) in *)
+(*      let constraints := ConstraintSet.add uc (snd G) in *)
+(*      (fst G, constraints). *)
+
+(* Definition repr (uctx : universe_context) : UContext.t := *)
+(*   match uctx with *)
+(*   | Monomorphic_ctx c => c *)
+(*   | Polymorphic_ctx c => c *)
+(*   | Cumulative_ctx c => CumulativityInfo.univ_context c *)
+(*   end. *)
+
+(* Definition add_global_constraints (uctx : universe_context) (G : t) : t *)
+(*   := match uctx with *)
+(*      | Monomorphic_ctx (inst, cstrs) => *)
+(*        let G := List.fold_left (fun s l => add_node l s) inst G in *)
+(*        ConstraintSet.fold add_constraint cstrs G *)
+(*      | Polymorphic_ctx _ => G *)
+(*      | Cumulative_ctx _ => G *)
+(*      end. *)
+
+
+
+Section Test.
+
+  Definition get_graph G0 := match G0 with
+                             | Some φ => φ
+                             | None => init_graph
+                             end.
+
+  Definition G0 := make_graph ConstraintSet.empty.
+  Check (eq_refl : G0 = Some _).
+  Definition G := get_graph G0.
+
+  Local Existing Instance default_checker_flags.
+
+  Check (eq_refl : check_leq G Universe.type0m Universe.type0 = true).
+  Check (eq_refl : check_lt G Universe.type0m Universe.type0 = true).
+  Check (eq_refl : check_lt G Universe.type0m Universe.type0m = false).
+  Check (eq_refl : check_lt G Universe.type0 Universe.type0m = false).
+  Check (eq_refl : check_lt G Universe.type0 Universe.type0 = false).
+  Check (eq_refl : no_universe_inconsistency G = true).
+
+  Definition ctrs0 := ConstraintSet.add (Level.Level "Top.0", Lt, Level.Level "Top.1")
+                                        (ConstraintSet.singleton (Level.Var 0, Lt, Level.Var 1)).
+  Definition G'0 := make_graph ctrs0.
+  Check (eq_refl : G'0 = Some _).
+  Definition G' := get_graph G'0.
+
+  Check (eq_refl : check_lt G' (Universe.make (Level.Level "Top.0")) (Universe.make (Level.Var 0)) = false).
+  Check (eq_refl : check_leq G' (Universe.make (Level.Level "Top.1")) (Universe.make (Level.lProp)) = false).
+  Check (eq_refl : check_leq G' (Universe.super (Level.Level "Top.1")) (Universe.make (Level.Level "Top.1")) = false).
+  Check (eq_refl : check_lt G' (Universe.make (Level.Level "Top.1")) (Universe.super (Level.Level "Top.1")) = true).
+  Check (eq_refl : check_lt G' (Universe.make (Level.Level "Top.1")) (Universe.make (Level.Level "Top.1")) = false).
+  Check (eq_refl : check_eq G' (Universe.make (Level.Level "Top.1")) (Universe.make (Level.Level "Top.1")) = true).
+  Check (eq_refl : no_universe_inconsistency G = true).
+
+  Check (eq_refl : check_lt G' (Universe.make (Level.Var 1)) (Universe.make (Level.Var 0)) = false).
+  Check (eq_refl : check_leq G' (Universe.make (Level.Var 0)) (Universe.make (Level.Var 1)) = true).
+  Check (eq_refl : check_lt G' (Universe.make (Level.Var 0)) (Universe.make (Level.Var 1)) = true).
+  Check (eq_refl : check_leq G' Universe.type1 Universe.type0 = false).
+  Check (eq_refl : check_lt G' Universe.type1 Universe.type1 = false).
+
+
+  Definition ctrs1 := ConstraintSet.add (Level.Var 1, Eq, Level.Var 2)
+                                        (ConstraintSet.add (Level.Var 2, Le, Level.lSet) ctrs0).
+  Definition G''0 := make_graph ctrs1.
+  Check (eq_refl : G''0 = Some _).
+  Definition G'' := get_graph G''0.
+
+  Check (eq_refl : no_universe_inconsistency G'' = false).
+
+End Test.
